compiler/src/ZLemmas.v
@@ -1,0 +1,103 @@
+Require Import Coq.ZArith.ZArith.
+Require Import Coq.micromega.Lia.
+Require Import coqutil.Z.BitOps.
+Require Import coqutil.Z.bitblast.
+
+Local Open Scope Z_scope.
+Local Open Scope bool_scope.
+
+Lemma mod_mod_remove_outer: forall a m n,
+    0 < m < n ->
+    n mod m = 0 ->
+    (a mod m) mod n = a mod m.
+Proof.
+  intros *. intros [A B] C. apply Z.mod_small.
+  pose proof (Z.mod_pos_bound a m A). lia.
+Qed.
+
+Lemma mod_mod_remove_inner: forall a m n,
+    0 < n < m ->
+    m mod n = 0 ->
+    (a mod m) mod n = a mod n.
+Proof.
+  intros. rewrite <- Znumtheory.Zmod_div_mod; try lia.
+  unfold Z.divide.
+  apply Zmod_divides in H0; [|lia].
+  destruct H0. subst m.
+  exists x. lia.
+Qed.
+
+Lemma div_mul_same: forall a b,
+    b <> 0 ->
+    a / b * b = a - a mod b.
+Proof.
+  intros.
+  pose proof (Zmod_eq_full a b H).
+  lia.
+Qed.
+
+Lemma sub_mod_exists_q: forall v m,
+    0 < m ->
+    exists q, v - v mod m = m * q.
+Proof.
+  intros.
+  apply (Zmod_divides (v - v mod m) m); [lia|].
+  rewrite <- Zminus_mod_idemp_l.
+  rewrite Z.sub_diag.
+  rewrite Z.mod_0_l; lia.
+Qed.
+
+Lemma shiftr_spec'': forall a n m : Z,
+    Z.testbit (Z.shiftr a n) m = (0 <=? m) &&  Z.testbit a (m + n).
+Proof.
+  intros.
+  destruct (Z.leb_spec 0 m).
+  - apply Z.shiftr_spec. assumption.
+  - rewrite Z.testbit_neg_r; trivial.
+Qed.
+
+Lemma shiftr_spec': forall a n m : Z,
+    Z.testbit (Z.shiftr a n) m = negb (m <? 0) &&  Z.testbit a (m + n).
+Proof.
+  intros.
+  destruct (Z.ltb_spec m 0).
+  - rewrite Z.testbit_neg_r; trivial.
+  - apply Z.shiftr_spec. assumption.
+Qed.
+
+Definition mask(x start eend: Z): Z :=
+  (x - x mod 2 ^ start) mod 2 ^ eend.
+
+Lemma mask_app_plus: forall v i j k,
+    0 <= i ->
+    i <= j ->
+    j <= k ->
+    mask v i j + mask v j k = mask v i k.
+Proof.
+  intros. unfold mask.
+  do 2 rewrite <- div_mul_same by (apply Z.pow_nonzero; lia).
+  rewrite <-! Z.land_ones by lia.
+  rewrite <-! Z.shiftl_mul_pow2 by lia.
+  rewrite <- or_to_plus; Z.bitblast.
+Qed.
+
+Ltac simpl_pow2_products :=
+  repeat match goal with
+         | |- context [ 2 ^ ?a * 2 ^ ?b ] =>
+           match isZcst a with true => idtac end;
+           match isZcst b with true => idtac end;
+           let c := eval cbv in (a + b) in change (2 ^ a * 2 ^ b) with (2 ^ c)
+         end.
+
+Ltac simpl_Zcsts :=
+  repeat match goal with
+         | |- context [?op ?a ?b] =>
+           match isZcst a with true => idtac end;
+           match isZcst b with true => idtac end;
+           match op with
+           | Z.add => idtac
+           | Z.sub => idtac
+           | Z.mul => idtac
+           end;
+           let r := eval cbv in (op a b) in change (op a b) with r
+         end.
